src/impl/TLS13.Impl.ConnectionState.Model.fsti
@@ -2715,7 +2715,8 @@ val lemma_received_alert_failure_state_evolves
                  }
                  (received_alert_failure_state st alert raw_received))
 
-val lemma_received_close_notify_state_evolves
+val lemma_received_close_notify_state_evolves_for_role
+  (role:CS.endpoint_role)
   (st:CS.connection_state)
   (raw_received:B.bytes)
   : Lemma
@@ -2723,7 +2724,7 @@ val lemma_received_close_notify_state_evolves
                 (st.CS.cs_model.CS.model_control == CS.ControlApplicationData \/
                  st.CS.cs_model.CS.model_control == CS.ControlClosing) /\
                 st.CS.cs_model.CS.model_config.CS.config_role ==
-                  CS.ClientEndpoint /\
+                  role /\
                 CS.event_raw_delta_legal
                   st.CS.cs_model
                   (CS.ConnNetworkEvent {
@@ -2747,6 +2748,41 @@ val lemma_received_close_notify_state_evolves
                      };
                    CS.delta_raw_sent = B.empty;
                    CS.delta_raw_received = raw_received;
+                 }
+                 (received_close_notify_state st raw_received))
+
+val lemma_received_close_notify_state_evolves
+  (st:CS.connection_state)
+  (raw_received:B.bytes)
+  : Lemma
+      (requires CS.connection_state_consistent st /\
+                (st.CS.cs_model.CS.model_control == CS.ControlApplicationData \/
+                 st.CS.cs_model.CS.model_control == CS.ControlClosing) /\
+                st.CS.cs_model.CS.model_config.CS.config_role ==
+                 CS.ClientEndpoint /\
+                CS.event_raw_delta_legal
+                 st.CS.cs_model
+                 (CS.ConnNetworkEvent {
+                   CL.message_direction = CL.Received;
+                   CL.message_value = M.TlsAlert T.CloseNotify;
+                 })
+                 B.empty
+                 raw_received)
+      (ensures CS.connection_state_evolves
+                 st
+                 (received_close_notify_state st raw_received) /\
+               CS.connection_state_consistent
+                 (received_close_notify_state st raw_received) /\
+               CS.legal_connection_delta
+                 st
+                 {
+                  CS.delta_event =
+                    CS.ConnNetworkEvent {
+                      CL.message_direction = CL.Received;
+                      CL.message_value = M.TlsAlert T.CloseNotify;
+                    };
+                  CS.delta_raw_sent = B.empty;
+                  CS.delta_raw_received = raw_received;
                  }
                  (received_close_notify_state st raw_received))
 
